Allow any integer-based type, not just 'int', in the following places:  * array indices (any dimension)  * array lengths (with new, any dimension)  * sequence indicies  * subsequence bounds (like sq[lo..hi])  * the new multiplicity in multiset update (m[t := multiplicity])  * subarray-to-sequence bounds (like a[lo..hi]) Note that for an array 'a', 'a.Length' is always an integer, so a comparison 'i < a.Length' still requires 'i' to be an integer, not any integer-based value.  Same for '|sq|' for a sequence 'sq'.

Source/Dafny/DafnyAst.cs
@@ -1220,12 +1220,13 @@ namespace Microsoft.Dafny {
   /// Arg is either Domain or Range, depending on what type it is.  Arg is the type
   /// one would use in an expression "x in C", whereas
   /// This proxy stands for one of:
-  ///   seq(T)       Domain,Range,Arg := int,T,T
-  ///   multiset(T)  Domain,Range,Arg := T,int,T
+  ///   seq(T)       Domain,Range,Arg := integer,T,T
+  ///   multiset(T)  Domain,Range,Arg := T,integer,T
   ///   if AllowMap, may also be:
   ///   map(T,U)     Domain,Range,Arg := T,U,T
   ///   if AllowArray, may also be:
-  ///   array(T)     Domain,Range,Arg := int,T,T
+  ///   array(T)     Domain,Range,Arg := integer,T,T
+  /// where "integer" refers to any integer-based numeric type.
   /// </summary>
   public class IndexableTypeProxy : RestrictedTypeProxy {
     public readonly bool AllowMap;
